too many failed attempts at debugging, docs

guarded/Inductives.v
@@ -1,42 +1,95 @@
-
+From MetaCoq.Guarded Require Import printers.
 From MetaCoq.Checker Require Import Checker. 
 From MetaCoq.Template Require Import utils BasicAst Ast AstUtils.
 From MetaCoq.Template Require Import Universes Environment Reflect LiftSubst. 
 From MetaCoq.Template.utils Require Import MCRTree. 
 
-From MetaCoq.Guarded Require Import Except Trace util.
+From MetaCoq.Guarded Require Import Except util.
 
 (** List of known defects:
   - The used MetaCoq reduction (from the Checker) does not handle projections.
   - constants and constant unfolding is not handled faithfully in MetaCoq. 
-    The guardedness checker will be able to unfold constants even when they should be opaque.
+    The guardedness checker will be able to unfold constants even when they should be opaque. 
+   - I don't currently understand the exact reasons why restrictions of subterm info flow through dependent matches is needed in some cases. I have documented what is restricted, but not why it is needed.
+
+  - there are likely tons of bugs (e.g. dB off-by-ones) in code which I couldn't properly test due to the slow reduction.
+
+  - effectively impossible to debug due to the a) slow-as-hell and lazy reduction employed by MetaCoq Run
+                                               b) string stuff is super slow in Coq 
+
+    When working with the trace monad, it is so slow in fact that its observational behaviour is equivalent to divergence on anything interesting :)
+    This is because the reduction employed by MetaCoq Run is a) lazy b) implements laziness in a seemingly very broken way where terms are copied around all the time (instead of using sharing).
+    Together with the fact that the checker needs to reduce all the time, the applications of the reduction function whd_all just get carried around with the HUGE representation of 
+    the environments Σ, Γ. 
+    And somehow, in most cases when the result is needed, it then takes forever to evaluate (even though there is a reduction path taking like two steps to reach a normal form by just unfolding the head constant... 
+
+    This leads to huge explosions in a) runtime and b) memory usage (it's very easy to fill 20GB of RAM with quite trivial examples thanks to the borked reduction strategy and the complete lack of structure sharing in MC's reduction).
+
+
+  - good luck with attempting to formally verify any of this stuff :DD
 *)
 
 
-(** Exceptions *)
+(** * Exceptions *)
+(** most of the code runs in a monad for handling errors/exceptions *)
 
 Notation loc := string (only parsing).
+
+(** ** Trace-monad based *)
+(** botched attempt at debugging Gallina by setting a bound on the number of bind steps in the monad and tracking [trace] info emitted in the code for easier debugging *)
+(** the bound is not very useful in practice due to lazy evaluation: the slow stuff happens at a totally different point (see the rant above) and is uncontrollable by limiting the number of steps *)
+(** in practice: not particularly useful as the string stuff like [bruijn_print] are evaluated lazily by MC Run and thus the huge unevaluated terms are passed around -- in practice, even one [trace] call with anything interesting thus leads to observational divergence *)
+
+(*From MetaCoq.Guarded Require Import Trace. *)
+
+(** to get MC to print the repr of arbitary stuff -- works because MetaCoq Run uses a very lazy evaluation strategy and does not reduce the thunk *)
+(*Definition thunk {A} (a : A) := "". *)
+(*Opaque thunk. [> nvm, tmEval does reduce it anyways <]*)
+
+(*Inductive guard_exc := *)
+  (*| ProgrammingErr (w : loc) (s : string)*)
+  (*| OtherErr (w : loc) (s : string)*)
+  (*| EnvErr (w: loc) (kn : kername) (s : string)*)
+  (*| IndexErr (w : loc) (s : string) (i : nat)*)
+  (*| GuardErr (w : loc) (s : string)*)
+  (*| TimeoutErr. *)
+
+(*max bind steps *)
+(*Definition max_steps := 500. *)
+(*Definition catchE := @catchE max_steps. *)
+(*Arguments catchE {_ _}. *)
+(*Definition catchMap := @catchMap max_steps _ TimeoutErr. *)
+(*Arguments catchMap {_ _}. *)
+  
+(*Instance: Monad (@TraceM guard_exc) := @trace_monad max_steps guard_exc TimeoutErr. *)
+(*Notation "'exc' A" := (@TraceM guard_exc A) (at level 100). *)
+(*Definition unwrap := @trc_unwrap.*)
+(*Arguments unwrap { _ _ _ _}. *)
+
+(*Instance: TrcUnwrap list := list_trc_unwrap max_steps TimeoutErr.*)
+
+
+
+
+(** * normal exception monad *)
 Inductive guard_exc := 
   | ProgrammingErr (w : loc) (s : string)
   | OtherErr (w : loc) (s : string)
   | EnvErr (w: loc) (kn : kername) (s : string)
   | IndexErr (w : loc) (s : string) (i : nat)
-  | GuardErr (w : loc) (s : string)
-  | TimeoutErr. 
+  | GuardErr (w : loc) (s : string).
+Notation "'exc' A" := (@excOn guard_exc A) (at level 100).
+(* just ignore traces *)
+Definition trace (t : string) : exc unit := ret tt.
 
-Definition max_steps := 250. 
-  
-Instance: Monad (@TraceM guard_exc) := @trace_monad max_steps guard_exc TimeoutErr. 
-Notation "'exc' A" := (@TraceM guard_exc A) (at level 100). 
-Definition unwrap := @trc_unwrap.
+Definition unwrap := @exc_unwrap.
 Arguments unwrap { _ _ _ _}. 
 
-Instance: TrcUnwrap list := list_trc_unwrap max_steps TimeoutErr.
 
 Notation "a == b" := (eqb a b) (at level 90). 
 Notation "a != b" := (negb(a==b)) (at level 90).
 
-(* As the guardedness checker reduces terms at many places before reducing, the key functions are not structurally recursive. 
+(** As the guardedness checker reduces terms at many places before reducing, the key functions are not structurally recursive. 
   We therefore disable the guardedness checker for this file. *)
 Unset Guard Checking. 
 
@@ -62,7 +115,7 @@ Definition constr_result_num_uniform (ctx : context) (num_pars : nat) (app : lis
     end
   in check_args app.
 
-(* Compute the number of parameters which can at most be uniform for an inductive. *)
+(** Compute the number of parameters which can at most be uniform for an inductive. *)
 Definition one_inductive_num_uniform (i : mind_specif) := 
   let ctors_hnf := ind_ctors_hnf i in
   let num_pars := (fst i).(ind_npars) in
@@ -74,7 +127,7 @@ Definition one_inductive_num_uniform (i : mind_specif) :=
   List.fold_left (fun acc c => min acc (one_constr c)) ctors_hnf num_pars. 
 
 
-(* Computes the number of uniform parameters of the mutual inductive definition [i]. 
+(** Computes the number of uniform parameters of the mutual inductive definition [i]. 
   Note: In Coq, for an inductive declaration 
     Inductive I X1 ... Xn : U := ...
   if Xi is non-uniform, then also Xj for j >= i are treated as non-uniform.
@@ -93,12 +146,12 @@ Implicit Types (kn : kername) (c: term).
 Definition whd_all Σ Γ t : exc term := 
   except (OtherErr "whd_all" "out of fuel") $ reduce_opt RedFlags.default Σ Γ default_fuel t. 
 
-(* β, ι, ζ weak-head reduction *)
+(** β, ι, ζ weak-head reduction *)
 Definition whd_βιζ Σ Γ t : exc term := 
   let redflags := RedFlags.mk true true true false false false in
   except (OtherErr "whd_βιζ" "out of fuel") $ reduce_opt redflags Σ Γ default_fuel t. 
 
-(* no let/ζ reduction *)
+(** no let/ζ reduction *)
 Definition whd_all_nolet Σ Γ t : exc term := 
   let redflags := RedFlags.mk true true false true true true in
   except (OtherErr "whd_all_nolet" "out of fuel") $ reduce_opt redflags Σ Γ default_fuel t. 
@@ -127,14 +180,14 @@ Definition get_const_value Σ kn : option term :=
   | None => None
   end.
 
-(* lookup a mutual inductive *)
+(** lookup a mutual inductive *)
 Definition lookup_mib Σ kn : exc mutual_inductive_body := 
   match lookup_env Σ kn with 
   | Some (InductiveDecl ind) => ret ind
   | _ => raise $ EnvErr "lookup_mib" kn "could not find inductive in global env"
   end.
 
-(* lookup an inductive *)
+(** lookup an inductive *)
 Definition lookup_mind_specif Σ (ind : inductive) : exc mind_specif := 
   mib <- lookup_mib Σ ind.(inductive_mind) ;;
   ib <- except (IndexErr "lookup_mind_specif" "invalid inductive index" ind.(inductive_ind)) $ 
@@ -142,7 +195,7 @@ Definition lookup_mind_specif Σ (ind : inductive) : exc mind_specif :=
   ret (mib, ib).
 
 
-(* if [t] evaluates to an application (weak-head) and the LHS is an inductive, return it together with the RHS (list) *)
+(** if [t] evaluates to an application (weak-head) and the LHS is an inductive, return it together with the RHS (list) *)
 Definition find_rectype Σ Γ t : exc inductive * Instance.t * list term:= 
   t <- whd_all Σ Γ t;; 
   let (t, l) := decompose_app t in 
@@ -152,27 +205,27 @@ Definition find_rectype Σ Γ t : exc inductive * Instance.t * list term:=
   end. 
 
 
-(* the same, but only if the rectype is an inductive or record (bifinite) *)
+(** the same, but only if the rectype is an inductive or record (bifinite) *)
 Definition find_inductive Σ Γ t := 
   '((i, u), l) <- find_rectype Σ Γ t;;
   '(mib, _) <- lookup_mind_specif Σ i;;
   if mib.(ind_finite) != CoFinite then ret ((i, u), l) 
     else raise $ OtherErr "find_inductive" "inductive is cofinite".
 
-(* only if coinductive *)
+(** only if coinductive *)
 Definition find_coinductive Σ Γ t := 
   '((i, u), l) <- find_rectype Σ Γ t;;
   '(mib, _) <- lookup_mind_specif Σ i;;
   if mib.(ind_finite) == CoFinite then ret ((i, u), l) 
     else raise $ OtherErr "find_coinductive" "inductive is not cofinite".
 
-(* push assumptions to the de Bruijn context *)
+(** push assumptions to the de Bruijn context *)
 Definition push_assumptions_context '(names, types) Γ := 
   (* we use fold_left, so the i-th element that is pushed to the context needs to be lifted by i *)
   let ctxt := map2_i (fun i name type => vass name (lift0 i type)) names types in
-  List.fold_left (fun acc assum => acc ,, assum) Γ ctxt. 
+  List.fold_left (fun acc assum => acc ,, assum) ctxt Γ. 
 
-(* [decompose_lam_assum Σ Γ ty] decomposes [ty] into a context of lambdas/lets and a remaining type, after reducing *)
+(** [decompose_lam_assum Σ Γ ty] decomposes [ty] into a context of lambdas/lets and a remaining type, after reducing *)
 Unset Guard Checking.
 Definition decompose_lam_assum Σ Γ := 
   let lamec_rec := fix lamec_rec Γ Γ0 ty {struct ty} :=
@@ -188,7 +241,7 @@ Definition decompose_lam_assum Σ Γ :=
     end
   in lamec_rec Γ [].
 
-(* [decompose_prod_assum Σ Γ ty] decomposes [ty] into a context of prods/lets and a remaining type, after reducing *)
+(** [decompose_prod_assum Σ Γ ty] decomposes [ty] into a context of prods/lets and a remaining type, after reducing *)
 Definition decompose_prod_assum Σ Γ := 
   let prodec_rec := fix prodec_rec Γ Γ0 ty {struct ty} := 
     ty_whd <- whd_all_nolet Σ Γ ty;;
@@ -200,13 +253,19 @@ Definition decompose_prod_assum Σ Γ :=
         let d := vdef x t ty in 
         prodec_rec (Γ ,, d) (Γ0 ,, d) body 
     | _ => 
-        (* try to reduce *)
-        ty_whd' <- whd_all Σ Γ ty_whd;;
-        if ty_whd == ty_whd' then ret (Γ0, ty_whd) else prodec_rec Γ Γ0 ty_whd'
+        (** try to reduce *)
+
+        (** TODO: commented reduction because this is ****ing slow /diverges *)
+        (** precisely: while the whd_all is fast due to laziness, the equality test takes forever (stopped after a few minutes) due to reducing the wrong redexes *)
+        (** this does already happen when e.g. ty = [tInd nat] (i.e., the whd_all could terminate in very few steps if the reduction strategy would pick the right redexes) *)
+        
+        (*ty_whd' <- whd_all Σ Γ ty_whd;;*)
+        (*if ty_whd == ty_whd' then ret (Γ0, ty_whd) else prodec_rec Γ Γ0 ty_whd'*)
+        ret (Γ0, ty)
     end 
   in prodec_rec Γ []. 
 
-(* [decompose_prod Σ Γ ty] decomposes [ty] into a context of prods and a remaining type, after reducing *)
+(** [decompose_prod Σ Γ ty] decomposes [ty] into a context of prods and a remaining type, after reducing *)
 Definition decompose_prod Σ Γ (t : term) : exc (context * term) := 
   let decrec := fix decrec Γ Γ0 t {struct t} := 
     t_whd <- whd_all Σ Γ t;;
@@ -218,7 +277,7 @@ Definition decompose_prod Σ Γ (t : term) : exc (context * term) :=
     end
   in decrec Γ [] t. 
 
-(* [decompose_lam_n_assum Σ Γ n t] decomposes [t] into a context of lambdas and lets. 
+(** [decompose_lam_n_assum Σ Γ n t] decomposes [t] into a context of lambdas and lets. 
   We expect [n] lambdas and also take all the lets up to the n-th lambda, but no more lets after the n-th lambda. *)
 Definition decompose_lam_n_assum Σ Γ n (t : term) : exc (context * term) := 
   let lamdec_rec := fix lamdec_rec Γ Γ0 n t {struct t} := 
@@ -238,16 +297,16 @@ Definition decompose_lam_n_assum Σ Γ n (t : term) : exc (context * term) :=
   in lamdec_rec Γ [] n t. 
 
 
-(* pseudo-reduction rule:
- * [hnf_prod_app env (Prod(_,B)) r] --> [B[r]]
- * with a HNF on [t] to produce a product. *)
+(** pseudo-reduction rule:
+  [hnf_prod_app env (Prod(_,B)) r] --> [B[r]]
+  with a HNF on [t] to produce a product. *)
 Definition hnf_prod_app Σ Γ t r : exc term := 
   t_whd <- whd_all Σ Γ t;;
   match t_whd with 
   | tProd _ _ body => ret $ subst10 r t
   | _ => raise $ OtherErr "hnf_prod_app" "need a product"
   end.
-(* use the previous reduction to apply a list of arguments [l] to [t]. *)
+(** use the previous reduction to apply a list of arguments [l] to [t]. *)
 Definition hnf_prod_apps Σ Γ t l : exc term := 
   List.fold_left (fun acc r => acc <- acc;; hnf_prod_app Σ Γ acc r) l (ret t). 
 
@@ -256,7 +315,7 @@ Definition mfix_names (fixp : mfixpoint term) := map dname fixp.
 Definition mfix_types (fixp : mfixpoint term) := map dtype fixp.
 Definition mfix_bodies (fixp : mfixpoint term) := map dbody fixp.
 
-(* [fold_term_with_binders g f n acc c] folds [f n] on the immediate
+(** [fold_term_with_binders g f n acc c] folds [f n] on the immediate
    subterms of [c] starting from [acc] and proceeding from left to
    right according to the usual representation of the constructions.
    It carries an extra data [n] (typically a lift
@@ -281,7 +340,7 @@ Definition fold_term_with_binders {X Y}(g : X -> X) (f : X -> Y -> term -> Y) (n
 
 
 
-(* check if a de Bruijn index in range 
+(** check if a de Bruijn index in range 
     n ... n + num -1 
   occurs in t *)
 (* TODO: might not handle evars/metas/casts correctly *)
@@ -299,7 +358,7 @@ Definition lookup_ind_subterms Σ (ind : inductive) :=
   '(_, oib) <- lookup_mind_specif Σ ind;;
   ret oib.(ind_recargs).
 
-(* check if a (function) type has an inductive co-domain *)
+(** check if a (function) type has an inductive co-domain *)
 Definition has_inductive_codomain Σ Γ t : exc bool := 
   '(abs_context, t') <- decompose_lam_assum Σ Γ t;;
   let Γ' := Γ ,,, abs_context in
@@ -332,14 +391,14 @@ Proof.
   intros [] []; constructor; congruence. 
 Defined.
 
-(* greatest lower bound/infimum of size information *)
+(** greatest lower bound/infimum of size information *)
 Definition size_glb s1 s2 := 
   match s1, s2 with 
   | Strict, Strict => Strict
   | _, _ => Loose
   end.
 
-(* possible specifications for a term:
+(** possible specifications for a term:
    - Not_subterm: when the size of a term is not related to the recursive argument of the fixpoint
    - Subterm: when the term is a subterm of the recursive argument
      the [wf_paths] argument specifies which subterms of the term are recursive 
@@ -366,10 +425,11 @@ Proof.
   intros [] []; unfold subterm_spec_eqb; finish_reflect. 
 Defined. 
 
-(* In contrast to the Boolean equality decider we get by eqb, this also checks equivalence if structural equality is failing by unfolding the recursive trees. *)
-Definition eq_wf_paths : wf_paths -> wf_paths -> bool := rtree_equal (eqb (A := recarg)). 
+(** In contrast to the Boolean equality decider we get by eqb, this also checks equivalence if structural equality is failing by unfolding the recursive trees. *)
+Definition eq_wf_paths a b: exc bool := 
+  except (OtherErr "eq_wf_paths" "rtree out of fuel") $ rtree_equal (eqb (A := recarg)) a b.
 
-(* Join the recarg info if compatible. *)
+(** Join the recarg info if compatible. *)
 Definition inter_recarg r1 r2 := 
   match r1, r2 with
   | Norec, Norec => Some Norec
@@ -382,15 +442,17 @@ Definition inter_recarg r1 r2 :=
 
 (** *** Operations on recursive arguments trees *)
 
-(* TODO: where exactly do we need intersections *)
-(* Intersection and equality test on [wf_paths]. *)
-Definition inter_wf_paths := rtree_inter (eqb (A := recarg)) inter_recarg Norec. 
-Definition incl_wf_paths := rtree_incl (eqb (A := recarg)) inter_recarg Norec. 
-Definition equal_wf_paths := rtree_equal (eqb (A := recarg)). 
+(** Intersection and equality test on [wf_paths]. Needed to restrict subterm information flowing through dependent matches.*)
+Definition inter_wf_paths a b : exc (option (rtree recarg)):= 
+  except (OtherErr "inter_wf_paths" "rtree out of fuel") $ rtree_inter (eqb (A := recarg)) inter_recarg Norec a b.
+Definition incl_wf_paths a b : exc bool := 
+  except (OtherErr "incl_wf_paths" "rtree out of fuel") $ rtree_incl (eqb (A := recarg)) inter_recarg Norec a b.
+Definition equal_wf_paths a b := 
+  except (OtherErr "equal_wf_paths" "rtree out of fuel") $ rtree_equal (eqb (A := recarg)) a b.
 
 Definition mk_norec := mk_node Norec []. 
 
-(* Given a recargs tree [t] representing for an inductive, get a list of trees for the arguments of the constructors. *)
+(** Given a recargs tree [t] representing for an inductive, get a list of trees for the arguments of the constructors. *)
 Definition wf_paths_constr_args_sizes t : exc (list (list wf_paths)) := 
   destruct_node t (fun ra constrs => 
     assert (match ra with Norec => false | _ => true end) $ ProgrammingErr "wf_paths_constr_args_sizes" "should not be called with Norec";;
@@ -399,21 +461,23 @@ Definition wf_paths_constr_args_sizes t : exc (list (list wf_paths)) :=
     ret l)
   (raise $ ProgrammingErr "wf_paths_constr_args_sizes" "expected node").
 
-(* Given a list of lists with the trees for the arguments (excluding parameters) of each constructor, 
+(** Given a list of lists with the trees for the arguments (excluding parameters) of each constructor, 
   construct the tree for a particular inductive type. 
   (This is not really a fully correct tree, as this is just the tree for one of the mutual inductives.) *)
 Definition mk_ind_paths rarg constr_arg_trees : wf_paths := 
   mk_node rarg (map (fun l => mk_node Norec l) constr_arg_trees). 
 
-(* Given a tree specifying the recursive structure of a term, generate a subterm spec. *)
-(* (used e.g. when matching on an element of inductive type) *)
-Definition spec_of_tree t := if eq_wf_paths t mk_norec then Not_subterm else Subterm Strict t. 
+(** Given a tree specifying the recursive structure of a term, generate a subterm spec. *)
+(** (used e.g. when matching on an element of inductive type) *)
+Definition spec_of_tree t : exc subterm_spec:= 
+  b <- eq_wf_paths t mk_norec;;
+  if b then ret $ Not_subterm else ret $ Subterm Strict t.
 
-(* Intersection of subterm specs. 
+(** Intersection of subterm specs. 
    Main use: when determining the subterm info for a match, we take the glb of the subterm infos for the branches.
 *)
-(* Dead_code is neutral element and Not_subterm least element. For Subterms, we intersect the recursive paths and the size. *)
-(* Example for the handling of Dead_code:
+(** Dead_code is neutral element and Not_subterm least element. For Subterms, we intersect the recursive paths and the size. *)
+(** Example for the handling of Dead_code:
     <<
       match n as n return n <> 0 -> nat with
       | 0 => fun H => match H with end
@@ -430,12 +494,13 @@ Definition subterm_spec_glb2 s1 s2 : exc subterm_spec :=
   | Not_subterm, _ => ret s1
   | _, Not_subterm => ret s2
   | Subterm a1 t1, Subterm a2 t2 => 
-      inter <- except (OtherErr "subterm_spec_glb2" "inter_wf_paths failed") $ inter_wf_paths t1 t2;;
+      inter <- inter_wf_paths t1 t2;;
+      inter <- except (OtherErr "subterm_spec_glb2" "inter_wf_paths failed: empty intersection") $ inter;;
       ret $ Subterm (size_glb a1 a2) inter
   end.
 
-(* Greatest lower bound of a list of subterm specs. *)
-(* Important: the neutral element is [Dead_code] -- for matches over empty types, we thus get [Dead_code]. *)
+(** Greatest lower bound of a list of subterm specs. *)
+(** Important: the neutral element is [Dead_code] -- for matches over empty types, we thus get [Dead_code]. *)
 Definition subterm_spec_glb (sl : list subterm_spec) : exc subterm_spec := 
   List.fold_left (fun acc s => acc <- acc;; subterm_spec_glb2 acc s) sl (ret Dead_code). 
 
@@ -444,19 +509,19 @@ Definition subterm_spec_glb (sl : list subterm_spec) : exc subterm_spec :=
 (** Environment to keep track of guardedness information *)
 Record guard_env := 
   { 
-    (* the local environment *)
+    (** the local environment *)
     loc_env : context;
-    (* de Bruijn index of the last fixpoint in this block (starting at 0) *)
-    (* i.e. in a block of [n] fixpoints, the dBs of the fixes are:
+    (** de Bruijn index of the last fixpoint in this block (starting at 0) *)
+    (** i.e. in a block of [n] fixpoints, the dBs of the fixes are:
         [rel_min_fix], ..., [rel_min_fix + n - 1]
     *)
     rel_min_fix : nat;
-    (* de Bruijn context containing subterm information *)
+    (** de Bruijn context containing subterm information *)
     guarded_env : list subterm_spec;
   }.
 Implicit Type (G : guard_env). 
 
-(* Make an initial guard_env after entering a fixpoint to check.
+(** Make an initial guard_env after entering a fixpoint to check.
   [recarg] is the index of the recursive argument, starting at 0. 
     e.g. for [fix r (n1 : nat) (n2 : nat) {struct n1} := ....] it would be 0.
   [tree] is the recursion tree for the inductive type of the recursive argument.
@@ -464,7 +529,7 @@ Implicit Type (G : guard_env).
 Definition init_guard_env Γ recarg tree :=
   {| 
     loc_env := Γ;
-    (* Rel 0 -> recursive argument, 
+    (** Rel 0 -> recursive argument, 
        Rel recarg -> first "proper" (non-recursive) argument,
        Rel (S recarg) -> last fixpoint in this block 
     *)
@@ -472,7 +537,7 @@ Definition init_guard_env Γ recarg tree :=
     guarded_env := [Subterm Loose tree]
   |}.
 
-(* Push a binder with name [na], type [type] and subterm specification [spec] *)
+(** Push a binder with name [na], type [type] and subterm specification [spec] *)
 Definition push_guard_env G '(na, type, spec) := 
   {|
     loc_env := G.(loc_env) ,, vass na type;
@@ -480,11 +545,11 @@ Definition push_guard_env G '(na, type, spec) :=
     guarded_env := spec :: G.(guarded_env);
   |}.
 
-(* add a new inner variable which is not a subterm *)
+(** add a new inner variable which is not a subterm *)
 Definition push_nonrec_guard_env G '(na, type) := 
   push_guard_env G (na, type, Not_subterm).
 
-(* Update the subterm spec of dB [i] to [new_spec] *)
+(** Update the subterm spec of dB [i] to [new_spec] *)
 Definition update_guard_spec G i new_spec := 
   {| 
     loc_env := G.(loc_env);
@@ -492,14 +557,14 @@ Definition update_guard_spec G i new_spec :=
     guarded_env := update_list G.(guarded_env) i new_spec 
   |}.
 
-(* lookup subterm information for de Bruijn index [p] *)
+(** lookup subterm information for de Bruijn index [p] *)
 Definition lookup_subterm G p := 
   match nth_error G.(guarded_env) p with 
   | Some spec => spec
   | None => Not_subterm
   end.
 
-(* push a local context as [Not_subterm]s *)
+(** push a local context as [Not_subterm]s *)
 Definition push_context_guard_env G Γ := 
   let n := length Γ in 
   {| 
@@ -508,7 +573,7 @@ Definition push_context_guard_env G Γ :=
     guarded_env := Nat.iter n (fun acc => Not_subterm :: acc) G.(guarded_env);
   |}. 
 
-(* push fixes to the guard env as [Not_subterm]s *)
+(** push fixes to the guard env as [Not_subterm]s *)
 Definition push_fix_guard_env G (mfix : mfixpoint term) := 
   let n := length mfix in
   {|
@@ -519,10 +584,10 @@ Definition push_fix_guard_env G (mfix : mfixpoint term) :=
 
 
 (** ** Stack *)
-(* A stack is used to maintain subterm information for elements which are (morally) applied to the term currently under observation, and which would really be applied if we could fully reduce with concrete values. 
+(** A stack is used to maintain subterm information for elements which are (morally) applied to the term currently under observation, and which would really be applied if we could fully reduce with concrete values. 
   [SClosure] is used for efficiency reasons: we don't want to compute subterm information for everything, so this is done on demand. It thus captures the term and the guardedness environment it's in.
   [SArg] represents subterm information for a term for which we actually have computed that information. *)
-(* Example where this is used: 
+(** Example where this is used: 
   << 
     match complex_fun n with 
     | 0 => fun t => ...
@@ -531,30 +596,30 @@ Definition push_fix_guard_env G (mfix : mfixpoint term) :=
   >>
   Here, the [fun t => ...] inside the match-branches would be checked with a stack having the subterm info for [k] at the head, as that term would really be applied to the [k].  
 *)
-(* (Note however that not all subterm information is allowed to flow through matches like that, see the functions below. ) *)
+(** (Note however that not all subterm information is allowed to flow through matches like that, see the functions below. ) *)
 Inductive stack_element := 
   | SClosure G (t : term)
   | SArg (s : subterm_spec). 
 
-(* Push a list of closures [l] with guard env [G] to the stack *)
+(** Push a list of closures [l] with guard env [G] to the stack *)
 Definition push_stack_closures G l stack := 
   List.fold_right (fun h acc => (SClosure G h) :: acc) l stack. 
 
-(* Push a list of args [l] to the stack *)
+(** Push a list of args [l] to the stack *)
 Definition push_stack_args l stack := 
   List.fold_right (fun h acc => SArg h :: acc) l stack. 
 
-(* Get the recarg the root node of [t] is annotated with. *)
+(** Get the recarg the root node of [t] is annotated with. *)
 Definition destruct_recarg (t : wf_paths) := destruct_node t (fun r _ => Some r) None. 
 
-(* Check that the recarg [r] is an [Mrec] or [Imbr] node with [ind]. *)
+(** Check that the recarg [r] is an [Mrec] or [Imbr] node with [ind]. *)
 Definition match_recarg_inductive (ind : inductive) (r : recarg) := 
   match r with
   | Norec => false
   | Mrec i | Imbr i => i == ind
   end.
 
-(* Add the types of mutual inductives as assumptions to the local context (the first inductive body at dB 0)
+(** Add the types of mutual inductives as assumptions to the local context (the first inductive body at dB 0)
   The inductive types are instantiated with the (uniform) parameters in [pars]. 
 *)
 Definition context_push_ind_with_params Σ Γ (mib : mutual_inductive_body) (pars : list term) : exc context := 
@@ -574,48 +639,10 @@ Definition context_push_ind_with_params Σ Γ (mib : mutual_inductive_body) (par
 
 
 (** ** Building recargs trees *)
-
-
-(* TODO: the following is not really what happens. 
-  We already have a tree with a suitable instantiation of nested inductive containers (the positivity checker uses a very similar function to compute it). 
-  The following stuff to compute a new tree is only ever used to restrict the flow of information through matches.. *)
-
-(** Nested inductives need special attention: to correctly handle matches (and subterms) on elements of a nested inductive type we are doing recursion over, the inner inductive type's parameters need to be properly instantiated with the outer inductive type. This is in particular the case for the recursive arguments tree. *)
-(** Example: rose trees
-   [Inductive rtree (X : Type) := rnode (l : list (rtree X)).]
-   When we check a fixpoint which is structural over [r : rtree X] and (after matching) [r] ≃ [rnode l], 
-    we want to be able to do recursive calls with elements of [l]. 
-   In order to obtain this subterm information when matching on [l], the recargs tree for the [list] type is instantiated with [rtree] beforehand. 
-
-                Rec 0 
-                 | 
-            Node (Mrec list_ind)
-        /                           \
-    Node Norec                   Node Norec
-                                /             \
-                            Node Norec    Param 0 0
-
-  is turned into
-
-                Rec 0 
-                 | 
-            Node (Imbr list_ind)
-        /                           \
-    Node Norec                   Node Norec
-                                /             \
-                            Param 1 0      Param 0 0
-
-  where the Param 1 1 references the node for [rtree] on the outside.
-  The full tree for [rtree] is then:
-
-              Rec 0
-                |
-        Node (Mrec rtree_ind)
-                | 
-            Node Norec
-                | 
-  [the instantiated tree for list] 
-    
+(** In some cases, we need to restrict the subterm information flowing through a dependent match.
+  In this case, we re-calculate an approximation of the recargs tree and intersect with it. *)
+(* TODO: I don't know at this point a) why these restrictions are needed for soundness
+                                    b) how the recargs tree calculated in the following differs from the one we already have statically computed -- for most purposes it seems to be identical (?) 
 *)
 
 (** To construct the recargs tree, the code makes use of [ra_env : list (recarg * wf_paths)], a de Bruijn context containing the recursive tree and the inductive for elements of an (instantiated) inductive type, and [(Norec, mk_norec)] for elements of non-inductive type.  
@@ -623,16 +650,15 @@ Definition context_push_ind_with_params Σ Γ (mib : mutual_inductive_body) (par
   Importantly, the recargs tree (of type wf_paths) may make references to other elements in the [ra_env] (via the [Param] constructor).
 *)
 
-
 (** Add the types of inner mutual inductives to a recargs environment. This is used in the context of nested inductives.
   Specifically, for the j-th inductive in the block, we add [(Imbr $ mkInd ind_kn j, Param 0 j)], i.e. an inner inductive with a direct recursive reference to the j-th inductive in the block. 
   The rest of the env is lifted accordingly.
   *)
 Definition ra_env_push_inner_inductives_with_params ra_env ind_kn ntypes := 
-  (* make inner inductive types (Imbr in the tree) with recursive references for the individual types *)
+  (** make inner inductive types (Imbr in the tree) with recursive references for the individual types *)
   let rc := rev $ mapi (fun i t => (Imbr (mkInd ind_kn i), t)) 
                        (mk_rec_calls (X := recarg) ntypes) in
-  (* lift the existing ra_env *)
+  (** lift the existing ra_env *)
   let ra_env := map (fun '(r, t) => (r, rtree_lift ntypes t)) ra_env in
   rc ++ ra_env. 
 
@@ -645,15 +671,15 @@ Definition lam_implicit_lift n t :=
   let lambda_implicit t := tLambda anon some_sort t in 
   Nat.iter n lambda_implicit (lift0 n t). 
 
-(* This removes global parameters of the inductive types in [constrs] (for nested inductive types only). *)
-(* for instance: if [constrs] is the list of [list] constructors, 
- * then we get back (roughly): [∀ X, (λ X, Rel 2) X;
- *                              ∀ X (x : X) (l : (λ X, Rel 3) X), (λ X, Rel 4) X]
- * i.e. we assume that at index 0 (at the outside) there is [list] instantiated with a parameter 
- * and we ignore the parameter X for the recursive occurrences of [list] in the constructor. *)
-(* Note : in the types in [constrs], the dBs 0... ntyps-1 refer to the mutual inductives. *)
-(* Now we substitute the references to these types. *)
-(* Effectively, this means that we just ignore the parameters and instead assume that at indices [0]... [ntypes-1], there are the inductive types already instantiated with some parameters. *)
+(** This removes global parameters of the inductive types in [constrs] (for nested inductive types only). *)
+(** for instance: if [constrs] is the list of [list] constructors, 
+  then we get back (roughly): [∀ X, (λ X, Rel 2) X;
+                               ∀ X (x : X) (l : (λ X, Rel 3) X), (λ X, Rel 4) X]
+  i.e. we assume that at index 0 (at the outside) there is [list] instantiated with a parameter 
+  and we ignore the parameter X for the recursive occurrences of [list] in the constructor. *)
+(** Note : in the types in [constrs], the dBs 0... ntyps-1 refer to the mutual inductives. *)
+(** Now we substitute the references to these types. *)
+(** Effectively, this means that we just ignore the parameters and instead assume that at indices [0]... [ntypes-1], there are the inductive types already instantiated with some parameters. *)
 Definition abstract_params_mind_constrs num_types num_params (constrs : list term) :=
   (* if there are no parameters, there is no abstracting to do *)
   if num_params == 0 then constrs
@@ -664,7 +690,7 @@ Definition abstract_params_mind_constrs num_types num_params (constrs : list ter
 
     map (subst0 make_abs) constrs.
 
-(* Move the first [n] prods of [c] into the context as elements of non-recursive type. *)
+(** Move the first [n] prods of [c] into the context as elements of non-recursive type. *)
 Fixpoint ra_env_decompose_prod Σ Γ (ra_env : list (recarg * wf_paths)) n (c : term) {struct c} : exc (context * list (recarg * wf_paths) * term) :=
   match n with 
   | 0 => ret (Γ, ra_env, c)
@@ -679,38 +705,39 @@ Fixpoint ra_env_decompose_prod Σ Γ (ra_env : list (recarg * wf_paths)) n (c : 
     end
   end.
 
-(* Create the recursive tree for a nested inductive [ind] applied to arguments [args]. *)
-(* In particular: starting from the tree [tree], we instantiate parameters suitably (with [args]) to handle nested inductives. *)
-(* [tree] is used to decide when to traverse nested inductives. *)
-(* [ra_env] is used to keep track of the subterm information of dB variables. 
+(** Create the recursive tree for a nested inductive [ind] applied to arguments [args]. *)
+(** In particular: starting from the tree [tree], we instantiate parameters suitably (with [args]) to handle nested inductives. *)
+(** [tree] is used to decide when to traverse nested inductives. *)
+(** [ra_env] is used to keep track of the subterm information of dB variables. 
    It need not bind all variables occurring in [t]: to unbound indices, we implicitly assign [Norec].*)
 Fixpoint build_recargs_nested Σ Γ (ra_env : list (recarg * wf_paths)) (tree : wf_paths) (ind: inductive) (args: list term) {struct args}: exc wf_paths := 
-  (* if the tree [tree] already disallows recursion, we don't need to go further *)
-  if equal_wf_paths tree mk_norec then ret tree else (
+  (** if the tree [tree] already disallows recursion, we don't need to go further *)
+  b_eq <- equal_wf_paths tree mk_norec;;
+  if b_eq : bool then ret tree else (
   '(mib, oib) <- lookup_mind_specif Σ ind;;
-  (* determine number of (non-) uniform parameters *)
+  (** determine number of (non-) uniform parameters *)
   let num_unif_params := num_uniform_params mib in
   let num_non_unif_params := mib.(ind_npars) - num_unif_params in
-  (* get the instantiations for the uniform parameters *)
-  (* Note that in Coq, all parameters after the first non-uniform parameter are treated as non-uniform -- thus we can just take a prefix of the list *)
+  (** get the instantiations for the uniform parameters *)
+  (** Note that in Coq, all parameters after the first non-uniform parameter are treated as non-uniform -- thus we can just take a prefix of the list *)
   let inst_unif := firstn num_unif_params args in
   let num_mut_inds := length mib.(ind_bodies) in
-  (* extend the environment with the inductive definitions applied to the parameters *)
+  (** extend the environment with the inductive definitions applied to the parameters *)
   Γ' <- context_push_ind_with_params Σ Γ mib inst_unif;;
-  (* do the same for the ra environment: 
+  (** do the same for the ra environment: 
     for the j-th inductive, 
     the recarg is Imbr (for the container), 
     the trees are direct recursive references [Param 0 j] *)
   let ra_env' := ra_env_push_inner_inductives_with_params ra_env ind.(inductive_mind) num_mut_inds in
 
-  (* lift the parameters we instantiate with by the number of types: 
+  (** lift the parameters we instantiate with by the number of types: 
     the dB layout we setup is: 
         [inductive types defined in the container of the nested ind], [the environment the parameters are assuming]
     Since we insert the inductive types when we use the parameters to instantiate the recargs tree, we thus have to lift the parameters by the number of mutual types of the container.
   *)
   let inst_unif_lifted := map (lift0 num_mut_inds) inst_unif in
 
-  (* In case of mutual inductive types, we use the recargs tree which was
+  (** In case of mutual inductive types, we use the recargs tree which was
     computed statically. This is fine because nested inductive types with
     mutually recursive containers are not supported -- meaning we need not instantiate in that case. 
     In the case that there are no mutual inductives, we use the argument tree [tree].*)
@@ -719,62 +746,62 @@ Fixpoint build_recargs_nested Σ Γ (ra_env : list (recarg * wf_paths)) (tree : 
     else unwrap $ map (fun oib => wf_paths_constr_args_sizes oib.(ind_recargs)) 
       mib.(ind_bodies));;
 
-  (* function: make the recargs tree for the [j]-th inductive in the block with body [oib].
-   * Essentially, we instantiate the corresponding recargs tree in [trees] with the parameters in [inst_unif]. *)
+  (** function: make the recargs tree for the [j]-th inductive in the block with body [oib].
+    Essentially, we instantiate the corresponding recargs tree in [trees] with the parameters in [inst_unif]. *)
   let mk_ind_recargs (j : nat) (oib : one_inductive_body) : exc wf_paths :=
-    (* get constructor types (with parameters), assuming that the mutual inductives are at [0]...[num_mut_inds-1]*)
+    (** get constructor types (with parameters), assuming that the mutual inductives are at [0]...[num_mut_inds-1]*)
     let constrs := map (fun '((_, c), _) => c) oib.(ind_ctors) in
-    (* abstract the parameters of the recursive occurrences of the inductive type in the constructor types *)
-    (* we assume that at indices [0]... [num_mut_inds-1], the inductive types are instantiated _with_ the parameters *)
+    (** abstract the parameters of the recursive occurrences of the inductive type in the constructor types *)
+    (** we assume that at indices [0]... [num_mut_inds-1], the inductive types are instantiated _with_ the parameters *)
     let abstracted_constrs := abstract_params_mind_constrs num_mut_inds num_unif_params constrs in
-    (* build the trees for the constructors, instantiated with the uniform parameters [inst_unif] *) 
+    (** build the trees for the constructors, instantiated with the uniform parameters [inst_unif] *) 
     paths <- unwrap $ mapi (fun k c => (* [k]-th constructor with abstracted type [c] *)
-        (* instantiate the abstracted constructor types with the parameters we are interested in. *)
+        (** instantiate the abstracted constructor types with the parameters we are interested in. *)
         c_inst <- hnf_prod_apps Σ Γ' c inst_unif_lifted;;
-        (* move non-uniform parameters into the context *) 
+        (** move non-uniform parameters into the context *) 
         '(Γ', ra_env', c') <- ra_env_decompose_prod Σ Γ' ra_env' num_non_unif_params c_inst;;
-        (* first fetch the trees for this constructor  *)
+        (** first fetch the trees for this constructor  *)
         constr_trees <- except (IndexErr "build_recargs_nested/mk_ind_recargs" "no tree for inductive" j) $ 
           nth_error trees j;;
         arg_trees <- except (IndexErr "build_recargs_nested/mk_ind_recargs" "no tree for constructor" k) $ 
           nth_error constr_trees k;; 
-        (* recursively build the trees for the constructor's arguments, potentially traversing nested inductives *)
+        (** recursively build the trees for the constructor's arguments, potentially traversing nested inductives *)
         build_recargs_constructors Σ Γ' ra_env' arg_trees c'
       ) abstracted_constrs;;
-      (* make the tree for this nested inductive *)
+      (** make the tree for this nested inductive *)
       ret $ mk_ind_paths (Imbr (mkInd ind.(inductive_mind) j)) paths
   in
-  (* create the trees for all the bodies *)
+  (** create the trees for all the bodies *)
   ind_recargs <- unwrap $ mapi mk_ind_recargs mib.(ind_bodies);;
-  (* now, given the bodies, make the mutual inductive trees *)
+  (** now, given the bodies, make the mutual inductive trees *)
   trees <- except (OtherErr "build_recargs_nested" "creating trees failed") $ mk_rec ind_recargs;;
-  (* return the tree for our particular inductive type *)
+  (** return the tree for our particular inductive type *)
   tree_ind <- except (IndexErr "build_recargs_nested" "created trees malformed" ind.(inductive_ind)) $ 
     nth_error trees ind.(inductive_ind);;
   ret tree_ind)
 
 (** Build the recargs tree for a term [t] -- in practice, [t] will be the type of a constructor argument. *)
-(* In the case that [t] contains nested inductive calls, [tree] is used to decide when to traverse nested inductives. *)
-(* [ra_env] is used to keep track of the subterm information of dB variables. 
+(** In the case that [t] contains nested inductive calls, [tree] is used to decide when to traverse nested inductives. *)
+(** [ra_env] is used to keep track of the subterm information of dB variables. 
    It need not bind all variables occurring in [t]: to unbound indices, we implicitly assign [Norec].*)
-(* This code is very close to check_positive in indtypes.ml, but does no positivity check and does not compute the number of recursive arguments. *)
-(* In particular, this code handles nested inductives as described above. *)
+(** This code is very close to check_positive in indtypes.ml, but does no positivity check and does not compute the number of recursive arguments. *)
+(** In particular, this code handles nested inductives as described above. *)
 with build_recargs Σ Γ (ra_env : list (recarg * wf_paths)) (tree : wf_paths) (t : term) {struct t}: exc wf_paths := 
   t_whd <- whd_all Σ Γ t;;
   let '(x, args) := decompose_app t_whd in
   match x with 
   | tProd na type body => 
-      (* simply enter the prod, adding the quantified element as assumption of non-recursive type (even though the type may in fact be inductive, for the purpose of determining the recargs tree of [t], this is irrelevant)*)
+      (** simply enter the prod, adding the quantified element as assumption of non-recursive type (even though the type may in fact be inductive, for the purpose of determining the recargs tree of [t], this is irrelevant)*)
       assert (args == []) (OtherErr "build_recargs" "tProd case: term is ill-typed");;
       let Γ' := Γ ,, vass na type in
       let ra_env' := (Norec, mk_norec) :: ra_env in
       build_recargs Σ Γ' ra_env' tree body
   | tRel k => 
-      (* free variables are allowed and assigned Norec *)
+      (** free variables are allowed and assigned Norec *)
       catchE (k_ra <- except (OtherErr "" "") $ nth_error ra_env k;; ret (snd k_ra)) 
             (fun _ => ret mk_norec)
   | tInd ind _ => 
-    (* if the given tree for [t] allows it (i.e. has an inductive as label at the root), we traverse a nested inductive *)
+    (** if the given tree for [t] allows it (i.e. has an inductive as label at the root), we traverse a nested inductive *)
     match destruct_recarg tree with 
     | None => raise $ OtherErr "build_recargs" "tInd case: malformed recargs tree"
     | Some (Imbr ind') | Some (Mrec ind') => 
@@ -787,7 +814,7 @@ with build_recargs Σ Γ (ra_env : list (recarg * wf_paths)) (tree : wf_paths) (
 
   
 
-(* [build_recargs_constructors Σ Γ ra_env trees c] builds a list of each of the constructor [c]'s argument's recursive structures, instantiating nested inductives suitably.  
+(** [build_recargs_constructors Σ Γ ra_env trees c] builds a list of each of the constructor [c]'s argument's recursive structures, instantiating nested inductives suitably.  
   We assume that [c] excludes parameters -- these should already be contained in the environment. 
 
   [trees] is a list of trees for the constructor's argument types, used to determine when to traverse nested inductive types.
@@ -821,17 +848,18 @@ with build_recargs_constructors Σ Γ (ra_env : list (recarg * wf_paths)) (trees
   in recargs_constr_rec Γ ra_env trees [] c. 
 
 
-(* [get_recargs_approx env tree ind args] builds an approximation of the recargs
+(** [get_recargs_approx env tree ind args] builds an approximation of the recargs
 tree for [ind], knowing [args] that are applied to it. 
 The argument [tree] is used to know when candidate nested types should be traversed, pruning the tree otherwise. *)
+(* TODO: figure out in which cases with nested inductives this isn't actually the identity *)
 Definition get_recargs_approx Σ Γ (tree : wf_paths) (ind : inductive) (args : list term) : exc wf_paths := 
   (* starting with ra_env = [] seems safe because any unbound tRel will be assigned Norec *)
   build_recargs_nested Σ Γ [] tree ind args. 
 
 
-(* [restrict_spec_for_match Σ Γ spec rtf] restricts the size information in [spec] to what is allowed to flow through a match with return-type function (aka predicate) [rtf] in environment (Σ, Γ). *)
-(* [spec] is the glb of the subterm specs of the match branches*)
-(* (this is relevant for cases where we go into recursion with the result of a match) *)
+(** [restrict_spec_for_match Σ Γ spec rtf] restricts the size information in [spec] to what is allowed to flow through a match with return-type function (aka predicate) [rtf] in environment (Σ, Γ). *)
+(** [spec] is the glb of the subterm specs of the match branches*)
+(** (this is relevant for cases where we go into recursion with the result of a match) *)
 (* TODO: how does get_recargs_approx play into this?*)
 Definition restrict_spec_for_match Σ Γ spec (rtf : term) : exc subterm_spec := 
   if spec == Not_subterm then ret Not_subterm
@@ -851,12 +879,13 @@ Definition restrict_spec_for_match Σ Γ spec (rtf : term) : exc subterm_spec :=
         match spec with 
         | Dead_code => ret Dead_code
         | Subterm size tree => 
-            (* intersect with approximation obtained by unfolding *)
+            (** intersect with approximation obtained by unfolding *)
             (* TODO: when does get_recargs_approx actually do something other than identity? *)
             recargs <- get_recargs_approx Σ Γ tree ind args;;
-            recargs <- except (OtherErr "restrict_spec_for_match" "intersection failed") $ inter_wf_paths tree recargs;;
+            recargs <- inter_wf_paths tree recargs;;
+            recargs <- except (OtherErr "restrict_spec_for_match" "intersection failed: empty") $ recargs;;
             ret (Subterm size recargs)
-        | _ => (* we already caught this case above *)
+        | _ => (** we already caught this case above *)
             raise $ OtherErr "restrict_spec_for_match" "this should not be reachable" 
         end
     | _ => ret Not_subterm
@@ -866,34 +895,35 @@ Definition restrict_spec_for_match Σ Γ spec (rtf : term) : exc subterm_spec :=
 (** ** Checking fixpoints *)
 
 
-(* Given a subterm spec for a term to match on, compute the subterm specs for the binders bound by a match in the individual branches. *)
-(* In [match c as z in ci y_s return P with |C_i x_s => t end]
+(** Given a subterm spec for a term to match on, compute the subterm specs for the binders bound by a match in the individual branches. *)
+(** In [match c as z in ci y_s return P with |C_i x_s => t end]
    [branches_specif Σ G c_spec ind] returns a list of [x_s]'s specs knowing
    [c_spec]. *)
-(* [ind] is the inductive we match on. *)
+ (** [ind] is the inductive we match on. *)
 Definition branches_binders_specif Σ G (discriminant_spec : subterm_spec) (ind : inductive) : exc list (list subterm_spec) := 
-  (* get the arities of the constructors (without lets, without parameters) *)
+  (** get the arities of the constructors (without lets, without parameters) *)
   constr_arities <- (
     '(_, oib) <- lookup_mind_specif Σ ind;;
     ret $ map snd oib.(ind_ctors));;
   unwrap $ mapi (fun i (ar : nat) => 
     match discriminant_spec return exc (list subterm_spec)  with 
     | Subterm _ tree => 
-        (* check if the tree refers to the same inductive as we are matching on *)
+        (** check if the tree refers to the same inductive as we are matching on *)
         recarg_info <- except (OtherErr "branches_binders_specif" "malformed tree") $ destruct_recarg tree;;
         if negb (match_recarg_inductive ind recarg_info) then
-          (* the tree talks about a different inductive than we are matching on, so all the constructor's arguments cannot be subterms  *)
+          (** the tree talks about a different inductive than we are matching on, so all the constructor's arguments cannot be subterms  *)
           ret $ tabulate (fun _ => Not_subterm) ar
         else 
-          (* get trees for the arguments of the i-th constructor *)
+          (** get trees for the arguments of the i-th constructor *)
           constr_args_sizes <- wf_paths_constr_args_sizes tree;;
           args_sizes <- except (IndexErr "branches_binders_specif" "no tree for constructor" i) $
             nth_error constr_args_sizes i;;
-          (* this should hopefully be long enough and agree with the arity of the constructor *)
+          (** this should hopefully be long enough and agree with the arity of the constructor *)
           assert (length args_sizes == ar) (OtherErr "branches_binders_specif" "number of constructor arguments don't agree");;
-          (* for each arg of the constructor: generate a strict subterm spec if they are recursive, otherwise Not_subterm. 
+          (** for each arg of the constructor: generate a strict subterm spec if they are recursive, otherwise Not_subterm. 
             These do also contain the recursive tree for that argument to enable nested matches. *)
-          ret $ map spec_of_tree args_sizes 
+          trees <- unwrap $ map spec_of_tree args_sizes;;
+          ret trees
     | Dead_code => 
         (* just propagate *)
         ret $ tabulate (fun _ => Dead_code) ar
@@ -904,7 +934,7 @@ Definition branches_binders_specif Σ G (discriminant_spec : subterm_spec) (ind 
     ) constr_arities.
 
 
-(* [subterm_specif Σ G stack t] computes the recursive structure of [t] applied to arguments with the subterm structures given by the [stack]. 
+(** [subterm_specif Σ G stack t] computes the recursive structure of [t] applied to arguments with the subterm structures given by the [stack]. 
   [G] collects subterm information about variables which are in scope. 
 *)
 Fixpoint subterm_specif Σ G (stack : list stack_element) t {struct t}: exc subterm_spec:= 
@@ -912,60 +942,59 @@ Fixpoint subterm_specif Σ G (stack : list stack_element) t {struct t}: exc subt
   let '(f, l) := decompose_app t_whd in 
   match f with 
   | tRel k => 
-      (* we abstract from applications: if [t] is a subterm, then also [t] applied to [l] is a subterm *)
+      (** we abstract from applications: if [t] is a subterm, then also [t] applied to [l] is a subterm *)
       ret $ lookup_subterm G k
   | tCase ind_relev rtf discriminant branches => 
       let '(ind, relev) := ind_relev in
-      (* push l to the stack *)
+      (** push l to the stack *)
       let stack' := push_stack_closures G stack l in
-      (* get subterm info for the discriminant *)
+      (** get subterm info for the discriminant *)
       discriminant_spec <- subterm_specif Σ G [] discriminant;;
-      (* get subterm info for the binders in the branches *)
+      (** get subterm info for the binders in the branches *)
       branches_binders_specs <- branches_binders_specif Σ G discriminant_spec (fst ind);;
-      (* determine subterm info for the full branches *)
+      (** determine subterm info for the full branches *)
       branches_specs <- unwrap $ mapi (fun i branch => 
         binder_specs <- except (IndexErr "subterm_specif" "branches_binders_specif result is too short" i) $ 
           nth_error branches_binders_specs i;;
         let stack_br := push_stack_args stack' binder_specs in
         subterm_specif Σ G stack_br branch) (map snd branches);;
-      (* take their glb -- in case of no branches, this yields [Dead_code] (absurd elimination) *)
+      (** take their glb -- in case of no branches, this yields [Dead_code] (absurd elimination) *)
       spec <- subterm_spec_glb branches_specs;;
-      (* restrict the subterm info according to the rtf *)
+      (** restrict the subterm info according to the rtf *)
       restrict_spec_for_match Σ G.(loc_env) spec rtf 
   | tFix mfix mfix_ind => 
       cur_fix <- except (IndexErr "subterm_specif" "invalid fixpoint index" mfix_ind) $ nth_error mfix mfix_ind;;
-      (* if the co-domain isn't an inductive, this surely can't be a subterm *)
+      (** if the co-domain isn't an inductive, this surely can't be a subterm *)
       ind_cod <- (has_inductive_codomain Σ G.(loc_env) cur_fix.(dtype));; 
       if negb ind_cod then ret Not_subterm 
       else 
         '(context, cur_fix_codomain) <- decompose_prod Σ G.(loc_env) cur_fix.(dtype);;
         let Γ' := G.(loc_env) ,,, context in 
-        (* if we can't find the inductive, it is not a subterm. *)
-        (* TODO is there actually a case where this is valid behvaviour? *)
+        (** if we can't find the inductive, just handle it as [Not_subterm]. *)
         catchMap (find_inductive Σ Γ' cur_fix_codomain) (fun _ => ret Not_subterm) $ fun '((ind, _), _) => 
         let num_fixes := length mfix in
-        (* get the recursive structure for the recursive argument's type *)
+        (** get the recursive structure for the recursive argument's type *)
         rectree <- lookup_ind_subterms Σ ind;;
-        (* push fixpoints to the guard env *)
+        (** push fixpoints to the guard env *)
         let G' := push_fix_guard_env G mfix in
-        (* we let the current fixpoint be a strict subterm *)
+        (** we let the current fixpoint be a strict subterm *)
         (* TODO: is this sound? why is it needed? nested fixes? *)
         let G' := update_guard_spec G' (num_fixes - mfix_ind) (Subterm Strict rectree) in
         let decreasing_arg := cur_fix.(rarg) in
         let body := cur_fix.(dbody) in 
-        (* number of abstractions (including the one for the decreasing arg) that the body is under *)
+        (** number of abstractions (including the one for the decreasing arg) that the body is under *)
         let num_abstractions := S decreasing_arg in
-        (* split into context up to (including) the decreasing arg and the rest of the body *)
+        (** split into context up to (including) the decreasing arg and the rest of the body *)
         '(context, body') <- decompose_lam_n_assum Σ G'.(loc_env) num_abstractions body;;
-        (* add the arguments as Not_subterm *)
+        (** add the arguments as Not_subterm *)
         let G'' := push_context_guard_env G' context in 
-        (* push the arguments [l] _ in guard env [G] _ *)
+        (** push the arguments [l] _ in guard env [G] _ *)
         let stack' := push_stack_closures G stack l in
 
-        (* before we go on to check the body: if there are enough arguments on the stack, 
+        (** before we go on to check the body: if there are enough arguments on the stack, 
           we can use the subterm information on the stack for the decreasing argument of 
           the nested fixpoint (instead of taking Not_subterm) *)
-        (* we check the body with an empty stack as it isn't directly applied to something*)
+        (** we check the body with an empty stack as it isn't directly applied to something*)
         if Nat.ltb (length stack') num_abstractions then subterm_specif Σ G'' [] body' else
           decreasing_arg_stackel <- except (IndexErr "subterm_specif" "stack' too short" decreasing_arg) $ 
             nth_error stack' decreasing_arg;;
@@ -974,7 +1003,7 @@ Fixpoint subterm_specif Σ G (stack : list stack_element) t {struct t}: exc subt
           subterm_specif Σ G'' [] body'
   | tLambda x ty body => 
      assert (l == []) (OtherErr "subterm_specif" "reduction is broken");;
-     (* get the subterm spec of what the lambda would be applied to (or Not_subterm if [stack] is empty)*)
+     (** get the subterm spec of what the lambda would be applied to (or Not_subterm if [stack] is empty)*)
      '(spec, stack') <- extract_stack_hd Σ stack;;
      subterm_specif Σ (push_guard_env G (x, ty, spec)) stack' body 
   | tEvar _ _ => 
@@ -982,8 +1011,8 @@ Fixpoint subterm_specif Σ G (stack : list stack_element) t {struct t}: exc subt
       (*ret Dead_code*)
       raise $ OtherErr "subterm_specif" "the guardedness checker does not handle evars"
   | tProj p t => 
-      (* compute the spec for t *)
-      (* TODO: why do we do this with the stack (instead of the empty stack)?
+      (** compute the spec for t *)
+      (** TODO: why do we do this with the stack (instead of the empty stack)?
         shouldn't _the result_ of the projection be applied to the elements of the stack?? *)
       t_spec <- subterm_specif Σ G stack t;;
       match t_spec with 
@@ -991,12 +1020,12 @@ Fixpoint subterm_specif Σ G (stack : list stack_element) t {struct t}: exc subt
           arg_trees <- wf_paths_constr_args_sizes paths;;
           match arg_trees with 
           | [arg_tree] => 
-              (* get the tree of the projected argument *)
+              (** get the tree of the projected argument *)
               let proj_arg := snd p in
               proj_arg_tree <- except (IndexErr "subterm_specif" "malformed recursive tree" proj_arg) $ 
                 nth_error arg_tree proj_arg;;
-              (* make a spec out of it *)
-              ret (spec_of_tree proj_arg_tree)
+                (** make a spec out of it *)
+              spec_of_tree proj_arg_tree
           | _ => raise $ OtherErr "subterm_specif" "projection on type having a number of constructors ≠ 1"
           end
       | Dead_code => ret Dead_code
@@ -1005,14 +1034,14 @@ Fixpoint subterm_specif Σ G (stack : list stack_element) t {struct t}: exc subt
   | _ => ret Not_subterm
   end
 
-(* given a stack element, compute its subterm specification *)
+(** given a stack element, compute its subterm specification *)
 with stack_element_specif Σ stack_el {struct stack_el} : exc subterm_spec := 
   match stack_el with 
   | SClosure G t => subterm_specif Σ G [] t
   | SArg spec => ret spec
   end
 
-(* get the subterm specification for the top stack element together with the rest of the stack*)
+(** get the subterm specification for the top stack element together with the rest of the stack*)
 with extract_stack_hd Σ stack {struct stack} : exc (subterm_spec * list stack_element) := 
   match stack with 
   | [] => ret (Not_subterm, [])
@@ -1021,16 +1050,16 @@ with extract_stack_hd Σ stack {struct stack} : exc (subterm_spec * list stack_e
       ret (spec, stack)
   end.
 
-(* Check that a term [t] with subterm spec [spec] can be applied to a fixpoint whose recursive argument has subterm structure [tree]*)
+(** Check that a term [t] with subterm spec [spec] can be applied to a fixpoint whose recursive argument has subterm structure [tree]*)
 Definition check_is_subterm spec tree := 
   match spec with 
   | Subterm Strict tree' => 
       (* TODO: find an example where the inclusion checking is needed -- probably with nested inductives? *)
       incl_wf_paths tree tree'
   | Dead_code => 
-      (* [spec] been constructed by elimination of an empty type, so this is fine *)
-      true
-  | _ => false
+      (** [spec] been constructed by elimination of an empty type, so this is fine *)
+      ret true
+  | _ => ret false
   end.
 
 
@@ -1049,7 +1078,7 @@ Definition check_is_subterm spec tree :=
       [Ti = ∀ y1 ... yn let z1 ... let zm := _ in IND t1 t2 ... tk]
     (where the prods and lets can appear in arbitrary permutations) and IND is an inductive type.
     In that case, we infer an approximate recargs tree for IND applied to t1 .... tk and 
-    intersect it with the subterm tree of xi in the stack. TODO: make this more precise
+    intersect it with the subterm tree of xi in the stack. 
   All other subterm information is truncated to Not_subterm. 
 
   TODO: why do we have these constraints given by the rtf? 
@@ -1084,17 +1113,17 @@ Definition filter_stack_domain Σ Γ (rtf : term) (stack : list stack_element) :
               match spec' with 
               | Not_subterm | Dead_code => ret elem (* don't restrict *)
               | Subterm s path => 
-                  (* intersect with an approximation of the unfolded tree for [ind] *)
+                  (** intersect with an approximation of the unfolded tree for [ind] *)
                   (* TODO : when does get_recargs_approx give something other than identity ? *)
                   recargs <- get_recargs_approx Σ Γ path ind ty_args;;
-                  path' <- except (OtherErr "filter_stack_domain" "intersection of trees failed") $ 
-                    inter_wf_paths path recargs;;
+                  path' <- inter_wf_paths path recargs;;
+                  path' <- except (OtherErr "filter_stack_domain" "intersection of trees failed: empty") path' ;;
                   (* update the recargs tree to [path'] *)
                   ret $ SArg (Subterm s path') 
               end
                  | _ => ret $ SArg Not_subterm (* if not an inductive, the subterm information is not propagated *) 
           end;;
-        (* NOTE: the Coq impl goes into recursion with Γ' ,, d. I believe that is wrong and have fixed it here. *)
+        (** NOTE: the Coq impl goes into recursion with Γ' ,, d. I believe that is wrong and have fixed it here. *)
         rest <- filter_stack (Γ ,, d) t0 stack';;
         ret (elem' :: rest)
       | _, _ => 
@@ -1103,7 +1132,7 @@ Definition filter_stack_domain Σ Γ (rtf : term) (stack : list stack_element) :
       end
     in filter_stack Γ' rtf_body stack.
 
-(* 
+(** 
   The main checker descending into the recursive structure of a term.
   Checks if [t] only makes valid recursive calls, with variables (and their subterm information) being tracked in the context [G].
 
@@ -1115,36 +1144,39 @@ Fixpoint check_rec_call (num_fixes : nat) (decreasing_args : list nat) trees
 Σ G (stack : list stack_element) (t : term) {struct t} : exc unit := 
   let check_rec_call' := check_rec_call num_fixes decreasing_args trees Σ in 
 
-  (* if [t] does not make recursive calls, then it is guarded: *)
+  (** if [t] does not make recursive calls, then it is guarded: *)
   if negb(rel_range_occurs G.(rel_min_fix) num_fixes t) then ret tt
   else 
     t_whd <- whd_βιζ Σ G.(loc_env) t;;
     (* FIXME: the guardedness checker will not be able to determine guardedness of this function since we wrap the match in there; thus l will not be determined as a subterm (as [] isn't) *)
     let (f, l) := decompose_app t_whd in  
+    (** NOTE : I have annotated some of the cases with conditions on guardedness, but these are partially incomplete as the [stack] of 'virtually applied' arguments complicates verbal descriptions quite a bit. 
+      The commented code is likely more informative. *)
     match f with 
     | tRel p =>
-        (* check if [p] is a fixpoint (of the block of fixpoints we are currently checking),i.e. we are making a recursive call *)
+        (** check if [p] is a fixpoint (of the block of fixpoints we are currently checking),i.e. we are making a recursive call *)
         if Nat.leb G.(rel_min_fix) p && Nat.ltb p (G.(rel_min_fix) + num_fixes) then
-          (* check calls in the argument list, initialized to an empty stack*)
+          (** check calls in the argument list, initialized to an empty stack*)
           _ <- list_iter (check_rec_call' G []) l;;
-          (* get the position of the invoked fixpoint in the mutual block *)
+          (** get the position of the invoked fixpoint in the mutual block *)
           let rec_fixp_index := G.(rel_min_fix) + num_fixes -1 - p in
-          (* get the decreasing argument of the recursive call *)
+          (** get the decreasing argument of the recursive call *)
           decreasing_arg <- except (IndexErr "check_rec_call" "invalid fixpoint index" rec_fixp_index) $ 
             nth_error decreasing_args rec_fixp_index;;
-          (* push the arguments as closures on the stack -- we don't infer their full subterm information yet *)
+          (** push the arguments as closures on the stack -- we don't infer their full subterm information yet *)
           (* NOTE : we don't really need to construct the updated stack here, but it seems cleaner *)
           let stack' := push_stack_closures G stack l in 
-          (* get the stack entry for the decreasing argument *)
+          (** get the stack entry for the decreasing argument *)
           z <- except (IndexErr "check_rec_call" "not enough arguments for recursive fix call" decreasing_arg) $ 
             nth_error stack' decreasing_arg;;
-          (* get the tree for the recursive argument type *)
+          (** get the tree for the recursive argument type *)
           recarg_tree <- except (IndexErr "check_rec_call" "no tree for the recursive argument" rec_fixp_index) $ 
             nth_error trees rec_fixp_index;;
-          (* infer the subterm spec of the applied argument *)
+          (** infer the subterm spec of the applied argument *)
           rec_subterm_spec <- stack_element_specif Σ z;;
-          (* verify that it is a subterm *)
-          if negb (check_is_subterm rec_subterm_spec recarg_tree) 
+          (** verify that it is a subterm *)
+          b_subt <-(check_is_subterm rec_subterm_spec recarg_tree);; 
+          if negb b_subt
           then 
             match z with 
             | SClosure z z' => raise $ GuardErr "check_rec_call" "illegal recursive call (could not ensure that argument is decresasing)"
@@ -1152,58 +1184,59 @@ Fixpoint check_rec_call (num_fixes : nat) (decreasing_args : list nat) trees
                 (* TODO: check if this is the right error *)
                 raise $ GuardErr "check_rec_call" "fix was partially applied"
             end
-          else ret tt
+          else  
+          ret tt
         else ret tt
 
-    (* Assume we are checking the fixpoint f. For checking [g a1 ... am]:
+    (** Assume we are checking the fixpoint f. For checking [g a1 ... am]:
       if - g = match d return rtf with | Ci xi1 ... xin => bi end
          - f is guarded with respect to the set of subterms S in a1 ... am
          - f is guarded with respect to the set of subterms S in the return-type function rtf
          - f is guarded with respect to the set of subterms S in the discriminant d
          - for each branch Ci xi1 ... xin => bi where S' := S ∪ { xij | the constructor Ci is recursive in the argument xij }:
-            f is guarded with respec to S' in the branch body
+            f is guarded with respect to S' in the branch body
             bi (virtually) applied to a1 ... am, where we restrict the subterm information of a1 ... am to 
             what is allowed to flow through the rtf
       then f is guarded with respect to the set of subterms S in [g a1 ... am].
     *)
     | tCase ind_nparams_relev rtf discriminant branches => 
-        (* match discriminant : ind return rtf with [branches] end *)
+        (** match discriminant : ind return rtf with [branches] end *)
         let '((ind, nparams), relev) := ind_nparams_relev in
-
         catchE (
-          (* check the arguments [l] it is applied to, the return-type function and the discriminant *)
+          (** check the arguments [l] it is applied to, the return-type function and the discriminant *)
           _ <- list_iter (check_rec_call' G []) l;;
           _ <- check_rec_call' G [] rtf;;
           _ <- check_rec_call' G [] discriminant;;
-          (* compute the recursive argument info for the binders of each branch by looking at the tree *)
+          (** compute the recursive argument info for the binders of each branch by looking at the tree *)
           discriminant_spec <- subterm_specif Σ G [] discriminant;; 
           case_branch_specs <- branches_binders_specif Σ G discriminant_spec ind;; 
-          (* push arguments on stack *)
+          (** push arguments on stack *)
           let stack' := push_stack_closures G stack l in
-          (* filter the stack to only contain the subterm info which is allowed to propagate through matches *)
+          (** filter the stack to only contain the subterm info which is allowed to propagate through matches *)
           stack' <- filter_stack_domain Σ G.(loc_env) rtf stack';;
-          (* check the branches of the matches *)
+          (** check the branches of the matches *)
           list_iteri (fun i '(_, branch) =>
               branch_spec <- except (IndexErr "check_rec_call" "branch specs too short" i) $ 
                 nth_error case_branch_specs i;;
-              (* push the rec arg specs for the binders introduced by the branch *)
+              (** push the rec arg specs for the binders introduced by the branch *)
               let stack_branch := push_stack_args stack' branch_spec in
-              (* check the branch *)
+              (** check the branch *)
               check_rec_call' G stack_branch branch) 
             branches
         )  
         (fun err => 
-          (* if the checking goes wrong, we can still try harder by reducing the match away if possible *)
+          (** if the checking goes wrong, we can still try harder by reducing the match away if possible *)
           discriminant <- whd_all Σ G.(loc_env) discriminant;;
           let '(hd, _) := decompose_app discriminant in
           match hd with 
           | tConstruct _ _ _ => 
-              (* just check the whole thing again with the reduced discriminant *)
+              (** just check the whole thing again with the reduced discriminant *)
               check_rec_call' G [] (mkApps (tCase ind_nparams_relev rtf discriminant branches) l)
           | _ => raise err
-          end)
+          end
+        )
 
-    (* Assume we are checking the fixpoint f. 
+    (** Assume we are checking the fixpoint f. 
        This implements the following rule for checking the term [g a1 ... am]:
        if - g = fix g (y1:T1)...(yp:Tp) {struct yp} := e 
           - f is guarded with respect to the set of subterms S in a1 ... am        
@@ -1215,29 +1248,29 @@ Fixpoint check_rec_call (num_fixes : nat) (decreasing_args : list nat) trees
         this_fix <- except (OtherErr "check_rec_call" "tFix: malformed fixpoint") $ nth_error mfix_inner fix_ind;;
         let decreasing_arg := rarg this_fix in 
         catchE (
-          (* check args *)
+          (** check args *)
           _ <- list_iter (check_rec_call' G []) l;;
-          (* check types *)
+          (** check types *)
           _ <- list_iter (check_rec_call' G []) (mfix_types mfix_inner);;
-          (* push arguments onto the stack *)
+          (** push arguments onto the stack *)
           let stack' := push_stack_closures G stack l in 
-          (* update the env with the rec. fixes *)
+          (** update the env with the rec. fixes *)
           let G' := push_fix_guard_env G mfix_inner in 
           list_iteri (fun j body => 
             if (fix_ind == j) && Nat.ltb decreasing_arg (length stack') then
-              (* we have subterm information for the decreasing arg on the stack *)
+              (** we have subterm information for the decreasing arg on the stack *)
               rec_arg_stackel <- except (ProgrammingErr "check_rec_call" "should be unreachable") $ 
                 nth_error stack' decreasing_arg;; 
-              (* compute the subterm spec for the recursive argument *)
+              (** compute the subterm spec for the recursive argument *)
               rec_arg_spec <- stack_element_specif Σ rec_arg_stackel;;
-              (* check the body of the fix after entering under the arguments and adding rec_arg_spec as the specification for [decreasing_arg] *)
+              (** check the body of the fix after entering under the arguments and adding rec_arg_spec as the specification for [decreasing_arg] *)
               check_nested_fix_body num_fixes decreasing_args trees Σ G' decreasing_arg rec_arg_spec body
             else 
-              (* just check the body with an empty stack *)
+              (** just check the body with an empty stack *)
               check_rec_call' G' [] body)
             (mfix_bodies mfix_inner))
           $ fun err => 
-            (* try to reduce the fix away by looking for a constructor in l[decreasing_arg] *)
+            (** try to reduce the fix away by looking for a constructor in l[decreasing_arg] *)
             if Nat.leb (length l) decreasing_arg then raise err else
             rec_arg_term <- except (ProgrammingErr "check_rec_call" "should be unreachable") $ 
               nth_error l decreasing_arg;;
@@ -1247,71 +1280,59 @@ Fixpoint check_rec_call (num_fixes : nat) (decreasing_args : list nat) trees
             | tConstruct _ _ _ => 
                 let before := firstn decreasing_arg l in 
                 let after := skipn (S decreasing_arg) l in
-                (* try again with the reduced recursive argument *)
+                (** try again with the reduced recursive argument *)
                 check_rec_call' G [] (mkApps (tFix mfix_inner fix_ind) (before ++ rec_arg_term :: after))
             | _ => raise err
             end
 
     | tConst kname univ => 
         if is_evaluable_const Σ kname then 
-          (* check the arguments *)
-          catchE (list_iter (check_rec_call' G []) l) $ fun _ => 
-          (* an error occurred, maybe it goes better if we apply the arguments reduce the constant? *)
+          (** check the arguments *)
+          catchE (list_iter (check_rec_call' G []) l) $ fun e => 
+          (** an error occurred, maybe it goes better if we apply the arguments and reduce the constant? *)
             val <- except (ProgrammingErr "check_rec_call" "constant lookup failed") $ get_const_value Σ kname;;
             check_rec_call' G stack (tApp val l)
         else 
-          (* just check the arguments without fallback *)
+          (** just check the arguments without fallback *)
           list_iter (check_rec_call' G []) l
 
-    (* Assume we are checking f. This implements the following rule for checking [g a1 ... an]:
-       if - g = λ x : t. b 
-          - f is guarded wrt the set of subterms S in t
-          - if f is guarded wrt the set of subterms S ∪ { 
-            TODO
-    *) 
     | tLambda x ty body =>
-        (* l is empty or reduction is broken *)
+        (** l is empty or reduction is broken *)
         _ <- assert (l == []) (OtherErr "check_rec_call" "tLambda : reduction is broken");;
-        (* check the type *)
+        (** check the type *)
         check_rec_call' G [] ty;;
-        (* we take the subterm spec at the head of the stack (corresponding to the element which will be applied to this lambda), or No_subterm if the stack is empty *)
+        (** we take the subterm spec at the head of the stack (corresponding to the element which will be applied to this lambda), or No_subterm if the stack is empty *)
         '(spec, stack') <- extract_stack_hd Σ stack;;
-        (* and check the body in the updated environment with the spec for this applied element *)
+        (** and check the body in the updated environment with the spec for this applied element *)
         check_rec_call' (push_guard_env G (x, ty, spec)) stack' body
 
 
     | tProd x ty body => 
-        (* the list [l] should be empty, otherwise the term is ill-typed *)
+        (** the list [l] should be empty, otherwise the term is ill-typed *)
         _ <- assert (l == []) (OtherErr "check_rec_call" "tProd: input term is ill-typed");;
-        (* moreover, the stack should be empty: 
-          We only ever put elements on the stack when we cannot reduce a match. 
-          Arguments which would be applied to a Prod would however not be allowed to flow through a match. 
-          TODO: this can't be the real reason: that information would still be on the stack, it would just be
-            Not_subterm.
-          *) 
         (*TODO Coq doesn't like the following check *)
         (*_ <- assert (stack == []) "tProd: stack should be empty";;*)
-        (* check the type *)
+        (** check the type *)
         check_rec_call' G [] ty;;
-        (* check the body: x is not a subterm *)
+        (** check the body: x is not a subterm *)
         check_rec_call' (push_nonrec_guard_env G (x, ty)) [] body
 
     | tCoFix mfix_inner fix_ind => 
-        (* check the arguments *)
+        (** check the arguments *)
         _ <- list_iter (check_rec_call' G []) l;;
-        (* check the types of the mfixes *)
+        (** check the types of the mfixes *)
         _ <- list_iter (check_rec_call' G []) (map dtype mfix_inner);;
-        (* check the bodies *)
+        (** check the bodies *)
         let G' := push_fix_guard_env G mfix_inner in
         list_iter (check_rec_call' G' []) (map dbody mfix_inner)
 
     | tInd _ _ | tConstruct _ _ _ => 
-        (* just check the arguments *)
+        (** just check the arguments *)
         list_iter (check_rec_call' G []) l
 
     | tProj p c =>
         catchE (
-          (* check arguments *)
+          (** check arguments *)
           _ <- list_iter (check_rec_call' G []) l;;
           check_rec_call' G [] c)
         $ fun exn => 
@@ -1335,36 +1356,36 @@ Fixpoint check_rec_call (num_fixes : nat) (decreasing_args : list nat) trees
         assert (l == []) $ OtherErr "check_rec_call" "tSort: ill-typed term"
 
     | tEvar _ _ => 
-        (* the RHS [l] is not checked because it is considered as the evar's context *)
-        (* NOTE: the guard checker is not really supposed to be dealing with evars -- it should be called on evar-free terms;
+        (** the RHS [l] is not checked because it is considered as the evar's context *)
+        (** NOTE: the guard checker is not really supposed to be dealing with evars -- it should be called on evar-free terms;
           see https://github.com/coq/coq/issues/9333#issuecomment-453235650*)
         raise $ OtherErr "check_rec_call" "guard checker should not be called on terms containing evars"
     | tApp _ _ | tLetIn  _ _ _ _ | tCast _ _ _ => raise (OtherErr "check_rec_call" "beta-zeta-iota reduction is broken")
     end
 
-(* Check the body [body] of a nested fixpoint with decreasing argument [decr] (dB index) and subterm spec [sub_spec] for the recursive argument.*)
-(* We recursively enter the body of the fix, adding the non-recursive arguments preceding [decr] to the guard env and finally add the decreasing argument with [sub_spec], before continuing to check the rest of the body *)
+(** Check the body [body] of a nested fixpoint with decreasing argument [decr] (dB index) and subterm spec [sub_spec] for the recursive argument.*)
+(** We recursively enter the body of the fix, adding the non-recursive arguments preceding [decr] to the guard env and finally add the decreasing argument with [sub_spec], before continuing to check the rest of the body *)
 with check_nested_fix_body (num_fixes : nat) (decreasing_args : list nat) trees
 Σ G (decr : nat) (sub_spec : subterm_spec) (body : term) {struct decr}: exc unit := 
   let check_rec_call' := check_rec_call num_fixes decreasing_args trees Σ in
-  (* reduce the body *)
+  (** reduce the body *)
   body_whd <- whd_all Σ G.(loc_env) body;;
   match body with 
   | tLambda x ty body => 
       _ <- check_rec_call' G [] ty;; 
       match decr with 
       | 0 =>
-        (* we have arrived at the recursive arg *)
+        (** we have arrived at the recursive arg *)
         check_rec_call' (push_guard_env G (x, ty, sub_spec)) [] body 
       | S n => 
-        (* push to env as non-recursive variable and continue recursively *)
+        (** push to env as non-recursive variable and continue recursively *)
         let G' := push_nonrec_guard_env G (x, ty) in  
         check_nested_fix_body num_fixes decreasing_args trees Σ G' n sub_spec body
       end
   | _ => raise $ OtherErr "check_nested_fix_body" "illformed inner fix body"
   end.
 
-(* Check if [def] is a guarded fixpoint body, with arguments up to (and including)
+(** Check if [def] is a guarded fixpoint body, with arguments up to (and including)
   the recursive argument being introduced in the context [G]. 
   [G] has been initialized with initial guardedness information on the recursive argument.
   [trees] is a list of recursive structures for the decreasing arguments of the mutual fixpoints.
@@ -1374,7 +1395,7 @@ Definition check_one_fix Σ G (recpos : list nat) (trees : list wf_paths) (def :
   check_rec_call (length recpos) recpos trees Σ G [] def.  
 
 
-(* Extract the [inductive] that [fixp] is doing recursion over (and check that the recursion is indeed over an inductive).
+(** Extract the [inductive] that [fixp] is doing recursion over (and check that the recursion is indeed over an inductive).
   Moreover give the body of [fixp] after the recursive argument and the environment (updated from [Γ])
   that contains the arguments up to (and including) the recursive argument (of course also the fixpoints). *)
 Definition inductive_of_mutfix Σ Γ (fixp : mfixpoint term) : exc (list inductive * list (context * term)):= 
@@ -1384,21 +1405,21 @@ Definition inductive_of_mutfix Σ Γ (fixp : mfixpoint term) : exc (list inducti
   let ftypes := mfix_types fixp in
   let fnames := mfix_names fixp in 
   let fbodies := mfix_bodies fixp in
-  (* push fixpoints to environment *)
+  (** push fixpoints to environment *)
   let Γ_fix := push_assumptions_context (fnames, ftypes) Γ in
   let nvect := map rarg fixp in 
 
-  (* Check the i-th definition [fixdef] of the mutual inductive block where k is the recursive argument, 
+  (** Check the i-th definition [fixdef] of the mutual inductive block where k is the recursive argument, 
     making sure that no invalid recursive calls are in the types of the first [k] arguments, 
     make sure that the recursion is over an inductive type, 
     and return that inductive together with the body of [fixdef] after the recursive arguement
     together with its context. *)
   let find_ind i k fixdef : exc (inductive * (context * term)):= 
-      (* check that a rec call to the fixpoint [fixdef] does not appear in the [k] first abstractions,
+      (** check that a rec call to the fixpoint [fixdef] does not appear in the [k] first abstractions,
         that the recursion is over an inductive, and 
         gives the inductive and the body + environment of [fixdef] after introducing the first [k] arguments *)
       let check_occur := fix check_occur Γ n (def : term) {struct def}: exc (inductive * (context * term)) := 
-        (* n is the number of lambdas we're under/aka the dB from which the mutual fixes are starting:
+        (** n is the number of lambdas we're under/aka the dB from which the mutual fixes are starting:
           n ... n + number_of_fixes - 1 *)
         def_whd <- whd_all Σ Γ def;;
         match def_whd with 
@@ -1406,23 +1427,23 @@ Definition inductive_of_mutfix Σ Γ (fixp : mfixpoint term) : exc (list inducti
             assert (negb(rel_range_occurs n number_of_fixes t)) 
               (GuardErr "inductive_of_mutfix" "bad occurrence of recursive call");;
             let Γ' := Γ ,, (vass x t) in
-            if n == k then (* becomes true once we have entered [k] inner lambdas*)
-              (* so now the rec arg should be at dB 0 and [t] is the type we are doing recursion over *)
-              (* get the inductive type of the fixpoint, ensuring that it is an inductive *)
+            if n == k then (** becomes true once we have entered [k] inner lambdas*)
+              (** so now the rec arg should be at dB 0 and [t] is the type we are doing recursion over *)
+              (** get the inductive type of the fixpoint, ensuring that it is an inductive *)
               '((ind, _), _) <- catchE (find_inductive Σ Γ t) (fun _ => raise $ GuardErr "inductive_of_mutfix" "recursion not on inductive");;
               '(mib, _) <- lookup_mind_specif Σ ind;;
               if mib.(ind_finite) != Finite then (* ensure that it is an inductive *)
                 raise $ GuardErr "inductive_of_mutfix" "recursion not on inductive"
               else
-                (* now return the inductive, the env after taking the inductive argument and all arguments before it, and the rest of the fix's body *)
+                (** now return the inductive, the env after taking the inductive argument and all arguments before it, and the rest of the fix's body *)
                 ret (ind, (Γ', body))
             else check_occur Γ' (S n) body
         | _ => 
-            (* not a lambda -> we do not have enough arguments and can't find the recursive one *)
+            (** not a lambda -> we do not have enough arguments and can't find the recursive one *)
             raise $ GuardErr "inductive_of_mutfix" "not enough abstractions in fix body" 
         end
       in 
-      (* check that recursive occurences are nice and extract inductive + fix body *)
+      (** check that recursive occurences are nice and extract inductive + fix body *)
       res <- check_occur Γ_fix 0 fixdef;; 
       let '(ind, _) := res in
       '(_, oib) <- lookup_mind_specif Σ ind;;
@@ -1430,32 +1451,32 @@ Definition inductive_of_mutfix Σ Γ (fixp : mfixpoint term) : exc (list inducti
       (* TODO some sprop checking for relevance *)
       ret res
   in 
-  (* now iterate this on all the fixpoints of the mutually recursive block *)
+  (** now iterate this on all the fixpoints of the mutually recursive block *)
   rv <- unwrap $ map2_i find_ind nvect fbodies;;
   trace "inductive_of_mutfix : leave";;
-  (* return the list of inductives as well as the fixpoint bodies in their context *)
+  (** return the list of inductives as well as the fixpoint bodies in their context *)
   ret (map fst rv : list inductive, map snd rv : list (context * term)).
 
 
 
 
-(* The entry point for checking fixpoints. 
+(** The entry point for checking fixpoints. 
   [Σ]: the global environment with all definitions used in [mfix]. 
   [Γ]: the local environment in which the fixpoint is defined.
   [mfix]: the fixpoint to check.
 *)
 Definition check_fix Σ Γ (mfix : mfixpoint term) : exc unit := 
-  (* check that the recursion is over inductives and get those inductives 
+  (** check that the recursion is over inductives and get those inductives 
     as well as the bodies of the fixpoints *)
   trace "enter check_fix";;
   '(minds, rec_defs) <- inductive_of_mutfix Σ Γ mfix;;
-  (* get the inductive definitions -- note that the mibs should all be the same*)
+  (** get the inductive definitions -- note that the mibs should all be the same*)
   specifs <- unwrap $ map (lookup_mind_specif Σ) minds;;
   let mibs := map fst specifs in
   let oibs := map snd specifs in
   let rec_trees := map (fun oib => oib.(ind_recargs)) oibs in
 
-  (* the environments with arguments introduced by the fix; 
+  (** the environments with arguments introduced by the fix; 
      for fix rec1 a1 ... an := .... with rec2 b1 ... bm := ... 
      the environment for rec1 would be 
       [an, ...., a1, rec2, rec1]
@@ -1463,18 +1484,16 @@ Definition check_fix Σ Γ (mfix : mfixpoint term) : exc unit :=
       [bm, ...., b1, rec2, rec1]
   *)
   let fix_envs := map fst rec_defs in     
-  let fix_bodies := map snd rec_defs in   (* the bodies under the respective [fix_envs] *)
+  let fix_bodies := map snd rec_defs in   (** the bodies under the respective [fix_envs] *)
   let rec_args := map rarg mfix in 
 
   _ <- unwrap $ mapi (fun i fix_body => 
     fix_env <- except (IndexErr "check_fix" "fix_envs too short" i) $ nth_error fix_envs i;;
     rec_tree <- except (IndexErr "check_fix" "rec_trees too short" i) $ nth_error rec_trees i;;
     rec_arg <- except (IndexErr "check_fix" "rec args too short" i) $ nth_error rec_args i;;
-    (* initial guard env *)
+    (** initial guard env *)
     let G := init_guard_env fix_env rec_arg rec_tree in
-    (* check the one fixpoint *)
+    (** check the one fixpoint *)
     check_one_fix Σ G rec_args rec_trees fix_body 
     ) fix_bodies;;
   ret tt.
-
-
