guarded/Trace.v
@@ -3,6 +3,10 @@ From MetaCoq.Template Require Import utils.
 Export MonadNotation.
 Require Import MetaCoq.Guarded.Except. 
 
+(** Trace Monad built on top of the exception monad for easier debugging. *)
+(** Provides means to limit the number of binds until timeout and to add trace information *)
+(** Sadly not very usable in practice due to slow Coq reduction. *)
+
 
 Section trace. 
   Context (max_steps : nat).
@@ -10,40 +14,42 @@ Section trace.
   Context (timeout : Y). 
 
   Definition trace_info := string. 
-  Definition TraceM A := nat (* number of steps on the clock *)
+  Definition TraceM A :=  bool (* timeout *)
+                        * nat (* number of steps on the clock *)
                         * list trace_info (* trace *)
                         * excOn Y A. (* error monad *)
 
   (* max steps handling is not totally accurate as we cannot pass the current number of steps into the function in bind, but anyways *)
   Instance trace_monad : Monad TraceM := 
     {| 
-      ret := fun T t => (0, [], ret t);
+      ret := fun T t => (false, 0, [], ret t);
       bind := fun T U x f => 
         match x with 
-        | (s, t, e) => 
+        | (b, s, t, e) => 
+            if b then (b, s, t, raise timeout) else 
             match e with 
             | inl e => 
                 match f e with 
-                | (s', t', e') => 
+                | (b', s', t', e') => 
                     let s'' := 1 + s' + s in
-                    if Nat.leb max_steps s'' then (s'', t' ++ t, raise timeout) 
-                      else (s'', t' ++ t, e')
+                    if b || Nat.leb max_steps s'' then (true, s'', t' ++ t, raise timeout) 
+                      else (false, s'', t' ++ t, e')
                 end
-            | inr err => (s, t, inr err)
+            | inr err => (false, s, t, inr err)
             end
         end
     |}. 
 
   (* emit a trace element *)
-  Definition trace (i : trace_info) : TraceM unit := (0, [i], ret tt). 
-  Definition step : TraceM unit := (1, [], ret tt). 
+  Definition trace (i : trace_info) : TraceM unit := (false, 0, [i], ret tt). 
+  Definition step : TraceM unit := (false, 1, [], ret tt). 
 
 
   (** Lifting of the primitive operations on the except monad *)
   Notation "'trc' A" := (@TraceM A) (at level 100).
 
-  Definition raise {X} (y : Y) : trc X := (0, [], Except.raise y).  
-  Definition except {X} (y: Y) (a : option X) : trc X := (0, [], Except.except y a). 
+  Definition raise {X} (y : Y) : trc X := (false, 0, [], Except.raise y).  
+  Definition except {X} (y: Y) (a : option X) : trc X := (false, 0, [], Except.except y a). 
 
   Class TrcUnwrap (Xl : Type -> Type) := trc_unwrap X : Xl (trc X) -> trc (Xl X).
   Arguments trc_unwrap {_ _ _}. 
@@ -58,10 +64,14 @@ Section trace.
     end.
   Instance list_trc_unwrap: TrcUnwrap list := @list_unwrap. 
 
-  Definition lift_exc {X} (a : excOn Y X) : trc X := (0, [], a).
+  Definition lift_exc {X} (a : excOn Y X) : trc X := (false, 0, [], a).
   Definition add_trace {Z} steps trace (a : trc Z) := 
     match a with 
-    | (steps', trace', z) => (steps + steps', trace' ++ trace, z)
+    | (b', steps', trace', z) => 
+        if b' then (b', steps', trace', z) else 
+          let steps'' := steps + steps' in
+          if Nat.leb max_steps steps'' then (true, steps'', trace' ++ trace, z)
+          else (false, steps + steps', trace' ++ trace, z)
     end.
 
   Definition assert (b : bool) (err : Y) : trc unit := 
@@ -69,25 +79,23 @@ Section trace.
 
   Definition catchE {X} (a : trc X) (f : Y -> trc X) : trc X := 
     match a with 
-    | (steps, trace, e) => 
+    | (true, steps, trace, e) => (true, steps, trace, e)
+    | (false, steps, trace, e) => 
         match e with 
-        | inl a => (steps, trace, e)
+        | inl a => (false, steps, trace, e)
         | inr e => 
             add_trace steps trace (f e)
         end
     end.
 
-  Definition catch {X} (a : trc X) (f : Y -> X) : X := 
-    match a with 
-    | (_, _, inr e) => f e
-    | (_, _, inl e) => e
-    end.
-
   Definition catchMap {X Z} (e : trc X) (f : Y -> trc Z) (g : X -> trc Z) : trc Z :=
     match e with
-    | (steps, trace, inr e) => 
+    | (true, steps, trace, inl e) => 
+        (true, steps, trace, inr timeout)
+    | (true, steps, trace, inr e) => (true, steps, trace, inr e) 
+    | (false, steps, trace, inr e) => 
         add_trace steps trace (f e)
-    | (steps, trace, inl a) => 
+    | (false, steps, trace, inl a) => 
         add_trace steps trace (g a)
     end.
 End trace.
@@ -100,6 +108,8 @@ Module example.
   | OtherErr (s : string). 
 
   Definition max_steps := 2. 
+  Definition catchE := @catchE max_steps. 
+  Arguments catchE {_ _}.
   
   Instance: Monad (@TraceM err) := @trace_monad max_steps err TimeoutErr. 
   Notation "'trc' A" := (@TraceM err A) (at level 100). 
