guarded/printers.v
@@ -1,4 +1,7 @@
-(* Adapted from  https://github.com/NeuralCoder3/metacoq/blob/unary-param/translations/de_bruijn_print.v *)
+(** * "Pretty" printers for terms and contexts. *)
+(** De facto not usable for debugging in MetaCoq due to slow reduction. :( *)
+(** Adapted from  https://github.com/NeuralCoder3/metacoq/blob/unary-param/translations/de_bruijn_print.v *)
+
 
 
 (*
@@ -85,55 +88,66 @@ Definition concatString (xs:list string) : string :=
 Print ident.
 Print tmQuoteInductive. *)
 
-Definition bruijn_print Σ := fix bruijn_print_aux (t:term) : string :=
+Definition lookup_ctx Γ n := 
+  match nth_error Γ n with
+  | Some decl => nameToString(decl.(decl_name).(binder_name))
+  | None => "u" :s (natToString n)
+  end.
+
+Definition bruijn_print Σ := fix bruijn_print_aux Γ (t:term) : string :=
   match t with
-  | tRel n => ("R" :s (natToString n))
+  | tRel n => 
+      ((lookup_ctx Γ n))
   | tVar ident => (ident)
   | tEvar n xs => "TODO:EVAR"
   | tSort univ => 
     "tSort ?"
   | tProd n t t2 => match n.(binder_name) with
-                   | nAnon => let s1 := bruijn_print_aux t in
-                              let s2 := bruijn_print_aux t2 in
+                   | nAnon => let s1 := bruijn_print_aux Γ t in
+                              let s2 := bruijn_print_aux (Γ ,, vass n t) t2 in
                              ("(":s append s1 (append ") -> " s2))
-                   | nNamed s => let s1 := bruijn_print_aux t in
-                                 let s2 := bruijn_print_aux t2 in
+                   | nNamed s => let s1 := bruijn_print_aux Γ t in
+                                 let s2 := bruijn_print_aux (Γ ,, vass n t) t2 in
                                 ("∀ (" +s s +s (" : "+s s1) +s "), " +s s2)
                    end
-  | tLambda s t t2 => let s1 := bruijn_print_aux t in
-                      let s2 := bruijn_print_aux t2 in
+  | tLambda s t t2 => let s1 := bruijn_print_aux Γ t in
+                      let s2 := bruijn_print_aux (Γ ,, vass s t) t2 in
                     ("λ ("+s match s.(binder_name) with
                         nAnon => "_"
                       | nNamed s => s
                       end
                      +s " : "+s s1+s"). "+s s2)
   | tLetIn name t1 t2 t3 =>
-    let s1 := bruijn_print_aux t1 in 
-    let s2 := bruijn_print_aux t2 in 
-    let s3 := bruijn_print_aux t3 in
+    let s1 := bruijn_print_aux Γ t1 in 
+    let s2 := bruijn_print_aux Γ t2 in 
+    let s3 := bruijn_print_aux (Γ ,, vdef name t1 t2) t3 in
     ("let "+s (nameToString name.(binder_name)) +s " := "+s s1 +s " : " +s s2 +s " in "+s linebreak +s s3)
   | tApp t1 t2 =>
-    let s1 := bruijn_print_aux t1 in
-    let s2 := List.fold_left (fun s t => let s2 := bruijn_print_aux t in (s +s s2 +s ";")) t2 "" in
+    let s1 := bruijn_print_aux Γ t1 in
+    let s2 := List.fold_left (fun s t => let s2 := bruijn_print_aux Γ t in (s +s s2 +s ";")) t2 "" in
     ("((" +s s1 +s ") [" +s s2 +s "])")
   | tConst kn ui => let (_,name) := kn in name
   | tInd ind ui => getInductiveName Σ ind.(inductive_mind) ind.(inductive_ind)
   | tConstruct ind n ui => getConstructName Σ ind.(inductive_mind) ind.(inductive_ind) n
   | tCase ((ind,n), _) p c brs =>
-    let sc := bruijn_print_aux c in
-    let sp := bruijn_print_aux p in
-    let sb := fold_left (fun sa x => match x with (n,t) => let st := bruijn_print_aux t in (sa +s " | ("+s(natToString n)+s") " +s st +s linebreak) end) brs "" in 
+    let sc := bruijn_print_aux Γ c in
+    let sp := bruijn_print_aux Γ p in
+    let sb := fold_left (fun sa x => match x with (n,t) => 
+        let st := bruijn_print_aux Γ t in 
+          (sa +s " | ("+s(natToString n)+s") " +s st +s linebreak) end) brs "" 
+    in 
     (linebreak +s "match (P:" +s (natToString n) +s ") "+s sc +s " return " +s sp +s " with" +s linebreak +s
             sb +s
              "end")
   | tProj p t => "TODO:Proj"
   | tFix mf n =>
+    let fix_ctx := Γ ,,, (map (fun d => vdef d.(dname) d.(dbody) d.(dtype)) mf) in
     (fix f xs := match xs with
                   nil => ""
                 | mfb::xs =>
                   let sr := f xs in
-          let stype := bruijn_print_aux (mfb.(dtype)) in 
-          let sbody := bruijn_print_aux (mfb.(dbody)) in
+          let stype := bruijn_print_aux Γ (mfb.(dtype)) in 
+          let sbody := bruijn_print_aux fix_ctx (mfb.(dbody)) in
           (linebreak +s "(fix "+s (nameToString mfb.(dname).(binder_name)) +s " : " +s stype +s " := " +s linebreak +s sbody +s ") "+s sr)
                 end
     ) mf
@@ -141,11 +155,24 @@ Definition bruijn_print Σ := fix bruijn_print_aux (t:term) : string :=
   end.
 
 
-Definition printTest := 
-  (forall (P:nat->Prop) (H0:P 0) (HS: forall n, P n -> P (S n)) (n:nat), P n).
+Definition print_context Σ Γ := 
+  let print_ctx := fix print_ctx Γ := 
+    match Γ with
+    | [] => ""
+    | decl :: Γ' =>
+        let na := nameToString (decl.(decl_name).(binder_name)) in
+        let ty := bruijn_print Σ Γ' decl.(decl_type) in
+        let bod := match decl.(decl_body) with | None => "[?]" | Some t => bruijn_print Σ Γ' t end in
+        "((" +s na +s " : " +s ty +s " := " +s bod +s "))" +s print_ctx Γ'
+    end
+  in "[[" +s print_ctx Γ +s "]]".
+        
+
+(*Definition printTest := *)
+  (*(forall (P:nat->Prop) (H0:P 0) (HS: forall n, P n -> P (S n)) (n:nat), P n).*)
 
 (*Definition test : TemplateMonad unit := *)
   (*mlet (Σ, t) <- tmQuoteRec printTest;;*)
-  (*s <- tmEval cbn (bruijn_print Σ t);;*)
+  (*s <- tmEval cbn (bruijn_print Σ [] t);;*)
   (*tmPrint  s. *)
 (*MetaCoq Run test. *)
